src/casemate-check-rocq/src/menhir_parser.mly
@@ -31,7 +31,7 @@
 
 trans:
     id= trans_id?
-    CPU COL cpu = NUM SCOL
+    CPU COL cpu = VAL
     data = trans_data
     AT
     src_loc = location
@@ -68,10 +68,10 @@ trans_data:
   //   CMSD_TRANS_HW_TLBI (
   //   let op, regime, shareability, level =
   //     match tlbi with
-  //     | "TLBI_vmalls12e1" -> (TLBIOp_VMALLS12, Regime_EL10, Shareability_NSH, TLBILevel_Any)
-  //     | "TLBI_vmalle1is" -> (TLBIOp_VMALL, Regime_EL10, Shareability_ISH, TLBILevel_Any)
-  //     | "TLBI_vmalls12e1is" -> (TLBIOp_VMALLS12, Regime_EL10, Shareability_ISH, TLBILevel_Any)
-  //     | "TLBI_vmalle1" -> (TLBIOp_VMALL, Regime_EL10, Shareability_NSH, TLBILevel_Any)
+  //     | "TLBI_vmalls12e1" -> (TLBIOp_VMALLS12, TLBI_REGIME_EL10, Shareability_NSH, TLBILevel_Any)
+  //     | "TLBI_vmalle1is" -> (TLBIOp_VMALL, TLBI_REGIME_EL10, Shareability_ISH, TLBILevel_Any)
+  //     | "TLBI_vmalls12e1is" -> (TLBIOp_VMALLS12, TLBI_REGIME_EL10, Shareability_ISH, TLBILevel_Any)
+  //     | "TLBI_vmalle1" -> (TLBIOp_VMALL, TLBI_REGIME_EL10, Shareability_NSH, TLBILevel_Any)
   //     | _ ->
   //         Printf.eprintf "Unsupported TLBI operation %s\n" tlbi;
   //         exit 1
@@ -90,10 +90,10 @@ trans_data:
   //   CMSD_TRANS_HW_TLBI (
   //     let op, regime, shareability, level =
   //       match tlbi with
-  //       | "TLBI_alle1is" -> (TLBIOp_ALL, Regime_EL10, Shareability_ISH, TLBILevel_Any)
-  //       | "TLBI_vale2is" -> (TLBIOp_VA, Regime_EL2, Shareability_ISH, TLBILevel_Last)
-  //       | "TLBI_vae2is" -> (TLBIOp_VA, Regime_EL2, Shareability_ISH, TLBILevel_Any)
-  //       | "TLBI_ipas2e1is" -> (TLBIOp_IPAS2, Regime_EL10, Shareability_ISH, TLBILevel_Any)
+  //       | "TLBI_alle1is" -> (TLBIOp_ALL, TLBI_REGIME_EL10, Shareability_ISH, TLBILevel_Any)
+  //       | "TLBI_vale2is" -> (TLBIOp_VA, TLBI_REGIME_EL2, Shareability_ISH, TLBILevel_Last)
+  //       | "TLBI_vae2is" -> (TLBIOp_VA, TLBI_REGIME_EL2, Shareability_ISH, TLBILevel_Any)
+  //       | "TLBI_ipas2e1is" -> (TLBIOp_IPAS2, TLBI_REGIME_EL10, Shareability_ISH, TLBILevel_Any)
   //       | _ ->
   //           Printf.eprintf "Unsupported TLBI operation %s\n" tlbi;
   //           exit 1
@@ -119,7 +119,7 @@ trans_data:
 write_types:
   | W {WMO_plain}
   | Wrel {WMO_release}
-  | Wpage {WMO_page}
+  // | Wpage {WMO_page}
 
 sysreg:
   | SYSREG_VTTBR {SYSREG_VTTBR}
