src/casemate-check-rocq/theories/transition.v
@@ -12,11 +12,11 @@ Require Import pgtable.
 
 (* Inductive SecurityState := SS_NonSecure | SS_Root | SS_Realm | SS_Secure. *)
 Inductive Regime := 
-  | Regime_EL3
-  | Regime_EL30
-  | Regime_EL2
-  | Regime_EL20
-  | Regime_EL10
+  | TLBI_REGIME_EL3
+  | TLBI_REGIME_EL30
+  | TLBI_REGIME_EL2
+  | TLBI_REGIME_EL20
+  | TLBI_REGIME_EL10
 .
 
 Inductive Shareability := 
@@ -128,15 +128,15 @@ Definition decode_tlbi_stage (td : trans_tlbi_data) : TLBI_stage_kind :=
 
 Definition decode_tlbi_regime (td : trans_tlbi_data) : Regime :=
   match td.(ttd_tlbi_kind) with
-  | TLBI_vmalls12e1 => Regime_EL10
-	| TLBI_vmalls12e1is => Regime_EL10
-	| TLBI_vmalle1is => Regime_EL10
-	| TLBI_alle1is => Regime_EL10
-	| TLBI_vmalle1 => Regime_EL10
-  | TLBI_vae2 => Regime_EL2
-	| TLBI_vale2is => Regime_EL2
-	| TLBI_vae2is => Regime_EL2
-	| TLBI_ipas2e1is => Regime_EL10
+  | TLBI_vmalle1is
+	| TLBI_vmalle1
+	| TLBI_ipas2e1is
+	| TLBI_vmalls12e1
+	| TLBI_vmalls12e1is
+	| TLBI_alle1is => TLBI_REGIME_EL10
+  | TLBI_vale2is
+	| TLBI_vae2is
+  | TLBI_vae2 => TLBI_REGIME_EL2
   end.
 
 Definition decode_tlbi_shootdown (td : trans_tlbi_data) : bool :=
@@ -175,7 +175,7 @@ Definition decode_tlbi_by_addr (td : trans_tlbi_data) : TLBI_op_by_addr_data :=
   let level := bv_and_64 td.(ttd_value) TLBI_TTL_MASK in
   let level_hint := 
     if (level b<? b4) then None 
-    else Some (bv_and_64 level b4) in
+    else Some (bv_and_64 level b3) in
 
   {|
     TOBAD_page := PA page;
@@ -191,11 +191,11 @@ Definition decode_tlbi_method (td : trans_tlbi_data) : TLBI_method :=
   | TLBI_vmalls12e1
 	| TLBI_vmalls12e1is
 	| TLBI_vmalle1is
-  | TLBI_vmalle1 => TLBI_by_input_addr (decode_tlbi_by_addr td)
+  | TLBI_vmalle1 => TLBI_by_addr_space (decode_tlbi_by_space_id td)
   | TLBI_vale2is
   | TLBI_vae2
   | TLBI_vae2is
-  | TLBI_ipas2e1is => TLBI_by_addr_space (decode_tlbi_by_space_id td)
+  | TLBI_ipas2e1is => TLBI_by_input_addr (decode_tlbi_by_addr td)
 	| TLBI_alle1is => TLBI_by_all
   end.
 
@@ -246,7 +246,6 @@ Inductive Barrier :=
 (* All those transitions will go in favor of ARM ISA description (except for hints) *)
 Inductive write_memory_order :=
   | WMO_plain
-  | WMO_page
   | WMO_release
 .
 
@@ -342,7 +341,7 @@ Definition clean_reachable_cb (ctx : pgtable_traverse_context) : casemate_model_
     match location.(sl_pte) with
     | None => Mreturn ctx.(ptc_state)
     | Some descriptor =>
-      match descriptor.(ged_state) with
+      match descriptor.(eed_state) with
       | SPS_STATE_PTE_INVALID_UNCLEAN _ =>
         Merror (CME_unclean_child ctx.(ptc_addr))
       | _ => Mreturn ctx.(ptc_state)
@@ -352,41 +351,40 @@ Definition clean_reachable_cb (ctx : pgtable_traverse_context) : casemate_model_
 
 Definition clean_reachable
   (map : table_data_t)
-  (descriptor : ghost_exploded_descriptor)
+  (descriptor : entry_exploded_descriptor)
   (cm : casemate_model_state):
   casemate_model_result :=
   traverse_pgt_from
-    descriptor.(ged_owner)
+    descriptor.(eed_owner)
     map.(next_level_table_addr)
-    descriptor.(ged_ia_region).(range_start)
-    (next_level descriptor.(ged_level))
-    descriptor.(ged_stage)
+    descriptor.(eed_ia_region).(range_start)
+    (next_level descriptor.(eed_level))
+    descriptor.(eed_stage)
     clean_reachable_cb
-    cm
-.
+    cm.
 
 Definition step_write_table_mark_children
   (tid : thread_identifier)
   (wmo : write_memory_order)
   (loc : sm_location)
   (val : u64)
-  (descriptor : ghost_exploded_descriptor)
+  (descriptor : entry_exploded_descriptor)
   (visitor_cb : pgtable_traverse_context -> casemate_model_result)
   (cm : casemate_model_state) :
   casemate_model_result :=
   if is_desc_valid val then
     (* Tests if the page table is well formed *)
-    match descriptor.(ged_pte_kind) with
+    match descriptor.(eed_pte_kind) with
     | PTER_PTE_KIND_TABLE map =>
       let st := clean_reachable map descriptor cm in
       let st := Mlog
         (Log "BBM: invalid clean->valid"%string (phys_addr_val loc.(sl_phys_addr))) st in
       Mupdate_state (traverse_pgt_from
-                        descriptor.(ged_owner)
+                        descriptor.(eed_owner)
                         map.(next_level_table_addr)
-                        descriptor.(ged_ia_region).(range_start)
-                        (next_level descriptor.(ged_level))
-                        descriptor.(ged_stage)
+                        descriptor.(eed_ia_region).(range_start)
+                        (next_level descriptor.(eed_level))
+                        descriptor.(eed_stage)
                         visitor_cb) st
     | _ => Mlog
           (Log "BBM: invalid clean->valid"%string (phys_addr_val loc.(sl_phys_addr))) (Mreturn cm)
@@ -409,10 +407,10 @@ Definition step_write_on_invalid
     | Some descriptor =>
       let descriptor := deconstruct_pte
           tid
-          descriptor.(ged_ia_region).(range_start)
-          val descriptor.(ged_level)
-          descriptor.(ged_owner)
-          descriptor.(ged_stage) in
+          descriptor.(eed_ia_region).(range_start)
+          val descriptor.(eed_level)
+          descriptor.(eed_owner)
+          descriptor.(eed_stage) in
       let new_loc := loc <| sl_val := val |> <| sl_pte := Some descriptor |> in
       let new_cm := cm <| cms_memory := <[ loc.(sl_phys_addr) := new_loc ]> cm.(cms_memory) |> in
       step_write_table_mark_children tid wmo loc val descriptor (mark_cb tid) new_cm
@@ -429,8 +427,7 @@ Definition step_write_on_invalid_unclean
   if is_desc_valid val then
     (Merror (CME_bbm_violation VT_valid_on_invalid_unclean loc.(sl_phys_addr)))
   else
-    Mreturn (cm <|cms_memory := <[loc.(sl_phys_addr) := loc <|sl_val := val|> ]> cm.(cms_memory) |>)
-.
+    Mreturn (cm <|cms_memory := <[loc.(sl_phys_addr) := loc <|sl_val := val|> ]> cm.(cms_memory) |>).
 
 Definition is_only_update_to_sw_bit (old new : u64) : bool :=
   (bv_and_64 old NOT_PTE_FIELD_UPPER_ATTRS_SW_MASK) b=? (bv_and_64 new NOT_PTE_FIELD_UPPER_ATTRS_SW_MASK)
@@ -444,8 +441,8 @@ Definition require_bbm
   match loc.(sl_pte) with
   | None => None (* PTE cannot be valid if it is not a PTE *)
   | Some old_descriptor =>
-    let new_descriptor := deconstruct_pte tid old_descriptor.(ged_ia_region).(range_start) val old_descriptor.(ged_level) old_descriptor.(ged_owner) old_descriptor.(ged_stage) in
-    match old_descriptor.(ged_pte_kind), new_descriptor.(ged_pte_kind) with
+    let new_descriptor := deconstruct_pte tid old_descriptor.(eed_ia_region).(range_start) val old_descriptor.(eed_level) old_descriptor.(eed_owner) old_descriptor.(eed_stage) in
+    match old_descriptor.(eed_pte_kind), new_descriptor.(eed_pte_kind) with
     | PTER_PTE_KIND_INVALID, _ | _, PTER_PTE_KIND_INVALID => Some false
     | PTER_PTE_KIND_TABLE _, _ | _, PTER_PTE_KIND_TABLE _ => Some true
     | PTER_PTE_KIND_MAP r1, PTER_PTE_KIND_MAP r2 =>
@@ -454,8 +451,7 @@ Definition require_bbm
       else
         Some (negb (is_only_update_to_sw_bit loc.(sl_val) val))
     end
-  end
-.
+  end.
 
 Definition step_write_valid_on_valid
   (tid : thread_identifier)
@@ -472,15 +468,14 @@ Definition step_write_valid_on_valid
       | None => (* This does not make sense because function is called on a pgt *)
         Merror (CME_internal_error IET_unexpected_none)
       | Some pte =>
-        let new_pte := deconstruct_pte tid pte.(ged_ia_region).(range_start) val pte.(ged_level) pte.(ged_owner) pte.(ged_stage) in
+        let new_pte := deconstruct_pte tid pte.(eed_ia_region).(range_start) val pte.(eed_level) pte.(eed_owner) pte.(eed_stage) in
         let loc := loc <| sl_val := val |> <| sl_pte := Some new_pte |> in
         Mreturn (insert_location loc cm)
       end
   | Some true =>
     (* Changing the descriptor is illegal *)
     Merror (CME_bbm_violation VT_valid_on_valid loc.(sl_phys_addr))
-  end
-.
+  end.
 
 Definition step_write_invalid_on_valid
   (tid : thread_identifier)
@@ -495,10 +490,10 @@ Definition step_write_invalid_on_valid
   | None => (* This does not make sense because function is called on a pgt *)
       Merror (CME_internal_error IET_unexpected_none)
   | Some descriptor =>
-    let new_desc := descriptor <| ged_state := (SPS_STATE_PTE_INVALID_UNCLEAN {| ai_invalidator_tid := tid; ai_old_valid_desc :=  old; ai_lis := LIS_unguarded; |}) |> in
+    let new_desc := descriptor <| eed_state := (SPS_STATE_PTE_INVALID_UNCLEAN {| ai_invalidator_tid := tid; ai_old_valid_desc :=  old; ai_lis := LIS_unguarded; |}) |> in
     let cm := (cm <| cms_memory := (<[ loc.(sl_phys_addr) := loc <|sl_pte := Some (new_desc)|> <| sl_val := val |> ]> cm.(cms_memory))|> ) in
     Mlog (Log "BBM: valid->invalid_unclean"%string (phys_addr_val loc.(sl_phys_addr)))
-    match descriptor.(ged_pte_kind) with
+    match descriptor.(eed_pte_kind) with
     | PTER_PTE_KIND_TABLE map =>
       let res := clean_reachable map descriptor cm in
       let res := Mlog (Log "invalidating a table descriptor"%string (phys_addr_val loc.(sl_phys_addr))) res in
@@ -506,8 +501,7 @@ Definition step_write_invalid_on_valid
       Mupdate_state (step_write_table_mark_children tid wmo loc val descriptor (mark_not_writable_cb tid)) res
     | _ => Mreturn cm
     end
-  end
-.
+  end.
 
 Definition step_write_on_valid
   (tid : thread_identifier)
@@ -529,35 +523,35 @@ Definition is_valid_state (st: sm_pte_state) : bool :=
   end
 .
 
-Definition drop_write_authorization_of_lock
+Definition drop_write_authorization
   (cpu : thread_identifier)
   (addr : phys_addr_t)
   (wmo : write_memory_order)
   (descriptor : u64)
-  (pte : ghost_exploded_descriptor)
+  (pte : entry_exploded_descriptor)
   (cm : casemate_model_state) : casemate_model_result :=
-  match get_lock_of_owner pte.(ged_owner) cm with
-  | None => Mreturn cm
-  | Some addr_lock =>
-    match lookup addr_lock cm.(cms_lock_state) with
+  match get_lock_of_owner pte.(eed_owner) cm with
+  | None => Merror CME_owner_not_associated
+  | Some lock_addr =>
+    match lookup lock_addr cm.(cms_lock_state) with
     | Some {| ls_tid := lock_owner; ls_write_authorization := auth |} =>
       if bool_decide (lock_owner = cpu) then
         match wmo with
-        | WMO_page | WMO_plain => (* check that the write is authorized, and then drop the authorization *)
+        | WMO_plain => (* check that the write is authorized, and then drop the authorization *)
           match auth with
           | WA_AUTHORIZED => 
             let new_lock_state := {| ls_tid := lock_owner; ls_write_authorization := WA_UNAUTHORIZED |} in
-            Mreturn (cm <| cms_lock_state := insert addr_lock new_lock_state cm.(cms_lock_state)|>)
+            Mreturn (cm <| cms_lock_state := insert lock_addr new_lock_state cm.(cms_lock_state)|>)
           | WA_UNAUTHORIZED =>
-            if (is_desc_valid descriptor) || is_valid_state pte.(ged_state) then
+            if (is_desc_valid descriptor) || is_valid_state pte.(eed_state) then
               Merror (CME_write_without_authorization addr)
             else
               let new_lock_state := {| ls_tid := lock_owner; ls_write_authorization := WA_UNAUTHORIZED |} in
-              Mreturn (cm <| cms_lock_state := insert addr_lock new_lock_state cm.(cms_lock_state)|>)
+              Mreturn (cm <| cms_lock_state := insert lock_addr new_lock_state cm.(cms_lock_state)|>)
           end
         | WMO_release => (* drop the authorization *)
           let new_lock_state := {| ls_tid := lock_owner; ls_write_authorization := WA_UNAUTHORIZED |} in
-          Mreturn (cm <| cms_lock_state := insert addr_lock new_lock_state cm.(cms_lock_state)|>)
+          Mreturn (cm <| cms_lock_state := insert lock_addr new_lock_state cm.(cms_lock_state)|>)
         end
       else
         Merror (CME_transition_without_lock addr)
@@ -565,7 +559,7 @@ Definition drop_write_authorization_of_lock
     end
   end.
 
-Definition drop_write_authorization
+Definition check_write_authorized
   (tid : thread_identifier)
   (wd : trans_write_data)
   (cm : casemate_model_state) :
@@ -582,37 +576,41 @@ Definition drop_write_authorization
         match location.(sl_pte) with
         | None => Mreturn cm
         | Some pte =>
-          if is_loc_thread_owned tid location cm then
-            Mreturn cm
-          else
-            drop_write_authorization_of_lock tid addr wmo val pte cm
+          match location.(sl_thread_owner) with
+          | Some thread_owner =>
+            if bool_decide (thread_owner = tid) then
+              Mreturn cm
+            else
+              Merror (CME_owned_pte_accessed_by_other_thread addr)
+          | None => drop_write_authorization tid addr wmo val pte cm
+          end
         end
-    end
-.
+    end.
 
-Definition step_write_aux
+Definition step_write
   (tid : thread_identifier)
   (wd : trans_write_data)
-  (cm : casemate_model_state) : casemate_model_result :=
-  let wmo := wd.(twd_mo) in
+  (cm : casemate_model_state) : 
+  casemate_model_result :=
+  let mo := wd.(twd_mo) in
   let val := wd.(twd_val) in
   let addr := wd.(twd_phys_addr) in
   if negb ((bv_and_64 (phys_addr_val addr) b7) b=? b0)
     then Merror CME_unaligned_write else
-  let new_st := drop_write_authorization tid wd cm in
+  let new_st := check_write_authorized tid wd cm in
   let write_update s :=
     match s !! addr with
     | Some (loc) =>
       match loc.(sl_pte) with
       | Some desc =>
         (* If we write to a page table, depending on its state, we update them  *)
-        match desc.(ged_state) with
+        match desc.(eed_state) with
         | SPS_STATE_PTE_VALID av =>
-            (step_write_on_valid tid wmo loc val s)
+            (step_write_on_valid tid mo loc val s)
         | SPS_STATE_PTE_INVALID_CLEAN av =>
-            (step_write_on_invalid tid wmo loc val s)
+            (step_write_on_invalid tid mo loc val s)
         | SPS_STATE_PTE_INVALID_UNCLEAN av =>
-            (step_write_on_invalid_unclean tid wmo loc val s)
+            (step_write_on_invalid_unclean tid mo loc val s)
         | SPS_STATE_PTE_NOT_WRITABLE =>
             (Merror (CME_write_on_not_writable addr))
         end
@@ -637,10 +635,9 @@ Definition step_write_aux
               |}
             ]> s.(cms_memory) |> in
                 Mreturn new_st
-          end
+    end
   in
-  Mupdate_state write_update new_st
-.
+  Mupdate_state write_update new_st.
 
 Function step_write_page
   (tid : thread_identifier)
@@ -659,18 +656,9 @@ Function step_write_page
         twd_val := wd.(twd_val);
       |}
     in
-    let res := Mupdate_state (step_write_aux tid sub_wd) res in
+    let res := Mupdate_state (step_write tid sub_wd) res in
     step_write_page tid wd res (offs - 1).
 Proof. lia. Qed.
-
-Definition step_write
-  (tid : thread_identifier)
-  (wd : trans_write_data)
-  (cm : casemate_model_state) : casemate_model_result :=
-  match wd.(twd_mo) with
-  | WMO_plain | WMO_release => step_write_aux tid wd cm
-  | WMO_page => step_write_page tid wd (Mreturn cm) z512
-  end.
 
 (** Mem init *)
 
@@ -752,19 +740,19 @@ Definition dsb_invalid_unclean_unmark_children
   let desc := (* This uses the old descriptor to rebuild a fresh old descriptor *)
     deconstruct_pte cpu_id ptc.(ptc_partial_ia) lis.(ai_old_valid_desc) ptc.(ptc_level) ptc.(ptc_root) ptc.(ptc_stage)
   in
-  match desc.(ged_pte_kind) with
+  match desc.(eed_pte_kind) with
   | PTER_PTE_KIND_TABLE map =>
     (* The children are clean, and not writable, otherwise, it would catch fire *)
-    traverse_pgt_from desc.(ged_owner) map.(next_level_table_addr) desc.(ged_ia_region).(range_start) (next_level desc.(ged_level)) desc.(ged_stage) (unmark_cb cpu_id) st
+    traverse_pgt_from desc.(eed_owner) map.(next_level_table_addr) desc.(eed_ia_region).(range_start) (next_level desc.(eed_level)) desc.(eed_stage) (unmark_cb cpu_id) st
   | _ => {| cmr_log  := nil; cmr_data := Ok _ _ st |}
   end.
 
 
 Definition new_pte_after_dsb
   (cpu_id : thread_identifier)
-  (pte : ghost_exploded_descriptor)
-  (kind : DxB) : ghost_exploded_descriptor :=
-  match pte.(ged_state) with
+  (pte : entry_exploded_descriptor)
+  (kind : DxB) : entry_exploded_descriptor :=
+  match pte.(eed_state) with
   | SPS_STATE_PTE_INVALID_UNCLEAN sst =>
     (* DSB has an effect on invalid unclean state only *)
     if negb (bool_decide (sst.(ai_invalidator_tid) = cpu_id)) then
@@ -773,19 +761,19 @@ Definition new_pte_after_dsb
       (* Otherwise, update the state invalid unclean sub-automaton *)
       match sst.(ai_lis) with
       | LIS_unguarded =>
-        pte <|ged_state := SPS_STATE_PTE_INVALID_UNCLEAN (sst <| ai_lis := LIS_dsbed |>) |>
+        pte <|eed_state := SPS_STATE_PTE_INVALID_UNCLEAN (sst <| ai_lis := LIS_dsbed |>) |>
       | LIS_dsbed => pte
       | LIS_dsb_tlbied =>
         match kind.(DxB_domain) with
         | MBReqDomain_InnerShareable | MBReqDomain_FullSystem =>
-          pte <| ged_state := SPS_STATE_PTE_INVALID_CLEAN {| aic_invalidator_tid := sst.(ai_invalidator_tid) |} |>
-              <| ged_pte_kind := PTER_PTE_KIND_INVALID |>
+          pte <| eed_state := SPS_STATE_PTE_INVALID_CLEAN {| aic_invalidator_tid := sst.(ai_invalidator_tid) |} |>
+              <| eed_pte_kind := PTER_PTE_KIND_INVALID |>
         | _ => pte
         end
       | LIS_dsb_tlbi_ipa =>
           match kind.(DxB_domain) with
           | MBReqDomain_InnerShareable | MBReqDomain_FullSystem =>
-            pte <|ged_state := SPS_STATE_PTE_INVALID_UNCLEAN (sst <|ai_lis := LIS_dsb_tlbi_ipa_dsb |>) |>
+            pte <|eed_state := SPS_STATE_PTE_INVALID_UNCLEAN (sst <|ai_lis := LIS_dsb_tlbi_ipa_dsb |>) |>
           | _ => pte
           end
       | _ => pte
@@ -810,7 +798,7 @@ Definition dsb_visitor
       let new_loc := (location <| sl_pte := Some new_pte |>) in
       let new_state := ctx.(ptc_state) <| cms_memory := <[ location.(sl_phys_addr) := new_loc ]> ctx.(ptc_state).(cms_memory) |> in
       let log :=
-        match pte.(ged_state), new_pte.(ged_state) with
+        match pte.(eed_state), new_pte.(eed_state) with
         | SPS_STATE_PTE_INVALID_UNCLEAN _ , SPS_STATE_PTE_INVALID_CLEAN _ =>
           Some (Log "BBM: invalid_unclean->invalid_clean"%string (phys_addr_val location.(sl_phys_addr)))
         | SPS_STATE_PTE_INVALID_UNCLEAN {| ai_lis := LIS_unguarded|} , SPS_STATE_PTE_INVALID_UNCLEAN {| ai_lis := _|} =>
@@ -821,7 +809,7 @@ Definition dsb_visitor
         end
       in
       let new_state :=
-        match pte.(ged_state), new_pte.(ged_state) with
+        match pte.(eed_state), new_pte.(eed_state) with
         | SPS_STATE_PTE_INVALID_UNCLEAN lis , SPS_STATE_PTE_INVALID_CLEAN _ =>
           dsb_invalid_unclean_unmark_children cpu_id new_loc lis
               (ctx <| ptc_state := new_state |> <|ptc_loc := Some new_loc|>)
@@ -884,7 +872,7 @@ Definition is_leaf (kind : pte_rec) : bool :=
   | _ => true
   end.
 
-Definition __get_tlbi_asid (td : TLBI_intermediate) : option addr_id_t :=
+Definition get_tlbi_asid (td : TLBI_intermediate) : option addr_id_t :=
   match td.(TI_method) with
   | TLBI_by_input_addr d => d.(TOBAD_asid)
   | TLBI_by_addr_space (PA addr_id) => Some (AID addr_id)
@@ -895,7 +883,7 @@ Fixpoint all_children_invalid_iter
   (idx : u64)
   (n_children : nat)
   (table_start : phys_addr_t)
-  (cm : casemate_model_state) :=
+  (cm : casemate_model_state) : bool :=
   match n_children with
   | O => true
   | S n_children =>
@@ -905,7 +893,7 @@ Fixpoint all_children_invalid_iter
       match child_loc.(sl_pte) with
       | None => false
       | Some child_pte_desc =>
-        match child_pte_desc.(ged_pte_kind) with
+        match child_pte_desc.(eed_pte_kind) with
         | PTER_PTE_KIND_INVALID =>
           all_children_invalid_iter (idx b+ b1) n_children table_start cm
         | _ => false
@@ -915,8 +903,8 @@ Fixpoint all_children_invalid_iter
     end
   end.
 
-Definition all_children_invalid (pte_desc : ghost_exploded_descriptor) (cm : casemate_model_state): bool :=
-  match pte_desc.(ged_pte_kind) with
+Definition all_children_invalid (pte_desc : entry_exploded_descriptor) (cm : casemate_model_state): bool :=
+  match pte_desc.(eed_pte_kind) with
   | PTER_PTE_KIND_TABLE table_data =>
     let table_start := table_data.(next_level_table_addr) in
     all_children_invalid_iter b0 512 table_start cm
@@ -936,11 +924,11 @@ Definition should_perform_tlbi
       match td.(TI_method) with
       | TLBI_by_input_addr d =>
         let tlbi_addr := bv_shiftl_64 (phys_addr_val d.(TOBAD_page)) b12 in
-        let ia_start := pte_desc.(ged_ia_region).(range_start) in
-        let ia_end := ia_start pa+ pte_desc.(ged_ia_region).(range_size) in
+        let ia_start := pte_desc.(eed_ia_region).(range_start) in
+        let ia_end := ia_start pa+ pte_desc.(eed_ia_region).(range_size) in
 
         (* If the PTE has valid children, the TLBI by VA is not enough *)
-        if (negb (is_leaf pte_desc.(ged_pte_kind)) && negb (all_children_invalid pte_desc ptc.(ptc_state))) then
+        if (negb (is_leaf pte_desc.(eed_pte_kind)) && negb (all_children_invalid pte_desc ptc.(ptc_state))) then
           Some false
 
         (* __should_perform_tlbi_matches_addr *)
@@ -948,15 +936,14 @@ Definition should_perform_tlbi
                   && (tlbi_addr b<? phys_addr_val ia_end)) then Some false
         
         (* __should_perform_tlbi_matches_level *)
-        else if ((negb (is_l3 pte_desc.(ged_level))) && d.(TOBAD_last_level_only)) then
+        else if ((negb (is_l3 pte_desc.(eed_level))) && d.(TOBAD_last_level_only)) then
           Some false
 
         else
           (* __should_perform_tlbi_matches_id *)
-          match td.(TI_regime), pte_desc.(ged_stage) with
-          | Regime_EL10, S2 =>
-            let roots := retrieve_roots_for_stage S2 ptc.(ptc_state).(cms_roots) in
-            match retrieve_root_for_baddr roots ptc.(ptc_root) with
+          match td.(TI_regime), pte_desc.(eed_stage) with
+          | TLBI_REGIME_EL10, S2 =>
+            match retrieve_root_for_baddr S2 ptc.(ptc_state).(cms_roots) ptc.(ptc_root) with
             | Some pte_root =>
               match get_current_vttbr cpu_id ptc.(ptc_state) with
               | Some vttbr => Some (bool_decide (pte_root.(r_id) = vttbr.(r_id)))
@@ -964,11 +951,10 @@ Definition should_perform_tlbi
               end
             | None => Some true
             end
-          | Regime_EL2, S1 =>
-            let roots := retrieve_roots_for_stage S1 ptc.(ptc_state).(cms_roots) in
-            match retrieve_root_for_baddr roots ptc.(ptc_root) with
+          | TLBI_REGIME_EL2, S1 =>
+            match retrieve_root_for_baddr S1 ptc.(ptc_state).(cms_roots) ptc.(ptc_root) with
             | Some pte_root =>
-              match __get_tlbi_asid td with
+              match get_tlbi_asid td with
               | Some asid => Some (bool_decide (pte_root.(r_id) = asid))
               | None => Some true
               end
@@ -977,10 +963,9 @@ Definition should_perform_tlbi
           | _, _ => Some true
           end
       | TLBI_by_addr_space addr_id =>
-        match td.(TI_regime), pte_desc.(ged_stage) with
-        | Regime_EL10, S2 =>
-          let roots := retrieve_roots_for_stage S2 ptc.(ptc_state).(cms_roots) in
-          match retrieve_root_for_baddr roots ptc.(ptc_root) with
+        match td.(TI_regime), pte_desc.(eed_stage) with
+        | TLBI_REGIME_EL10, S2 =>
+          match retrieve_root_for_baddr S2 ptc.(ptc_state).(cms_roots) ptc.(ptc_root) with
           | Some pte_root =>
             match get_current_vttbr cpu_id ptc.(ptc_state) with
             | Some vttbr => Some (bool_decide (pte_root.(r_id) = vttbr.(r_id)))
@@ -988,11 +973,10 @@ Definition should_perform_tlbi
             end
           | None => Some true
           end
-        | Regime_EL2, S1 =>
-          let roots := retrieve_roots_for_stage S1 ptc.(ptc_state).(cms_roots) in
-          match retrieve_root_for_baddr roots ptc.(ptc_root) with
+        | TLBI_REGIME_EL2, S1 =>
+          match retrieve_root_for_baddr S1 ptc.(ptc_state).(cms_roots) ptc.(ptc_root) with
           | Some pte_root =>
-            match __get_tlbi_asid td with
+            match get_tlbi_asid td with
             | Some asid => Some (bool_decide (pte_root.(r_id) = asid))
             | None => Some true
             end
@@ -1008,8 +992,8 @@ Definition should_perform_tlbi
 
 Definition step_pte_on_tlbi_after_dsb (td: TLBI_intermediate) : option LIS :=
   match td.(TI_regime) with
-  | Regime_EL2 => Some LIS_dsb_tlbied
-  | Regime_EL10 =>
+  | TLBI_REGIME_EL2 => Some LIS_dsb_tlbied
+  | TLBI_REGIME_EL10 =>
     match td.(TI_stage) with
     | TLBI_OP_stage1 => Some LIS_dsbed (* no effect*)
     | TLBI_OP_stage2 => Some LIS_dsb_tlbi_ipa
@@ -1020,7 +1004,7 @@ Definition step_pte_on_tlbi_after_dsb (td: TLBI_intermediate) : option LIS :=
 
 Definition step_pte_on_tlbi_after_tlbi_ipa (td: TLBI_intermediate) : option LIS :=
   match td.(TI_regime) with
-  | Regime_EL10 =>
+  | TLBI_REGIME_EL10 =>
       match td.(TI_stage) with
       | TLBI_OP_stage1 | TLBI_OP_both_stages => Some LIS_dsb_tlbied
       | TLBI_OP_stage2 => Some LIS_dsb_tlbi_ipa_dsb
@@ -1047,7 +1031,7 @@ Definition tlbi_visitor
         | None => Merror (CME_internal_error IET_unexpected_none)
           (* This cannot happen (otherwise, should_perform_tlbi would be false) *)
         | Some exploded_desc =>
-          match exploded_desc.(ged_state) with
+          match exploded_desc.(eed_state) with
           | SPS_STATE_PTE_INVALID_UNCLEAN ai =>
             (* If the CPU that does the transformation is not the one that initiated the invalidation, do nothing *)
             if bool_decide (cpu_id = ai.(ai_invalidator_tid)) then
@@ -1071,7 +1055,7 @@ Definition tlbi_visitor
                   end
                 in
                 (* Write the new sub-state in the global automaton *)
-                let new_loc := location <| sl_pte := Some (exploded_desc <|ged_state := SPS_STATE_PTE_INVALID_UNCLEAN (ai <| ai_lis := new_substate|>) |>)|> in
+                let new_loc := location <| sl_pte := Some (exploded_desc <|eed_state := SPS_STATE_PTE_INVALID_UNCLEAN (ai <| ai_lis := new_substate|>) |>)|> in
                 let new_mem := ptc.(ptc_state) <| cms_memory := <[location.(sl_phys_addr) := new_loc]> ptc.(ptc_state).(cms_memory)|> in
                 log (Mreturn new_mem)
               end
@@ -1085,19 +1069,23 @@ Definition tlbi_visitor
     end
   end.
 
-Definition step_tlbi (tid : thread_identifier) (td : trans_tlbi_data) (cm : casemate_model_state) : casemate_model_result :=
+Definition step_tlbi 
+  (tid : thread_identifier)
+  (td : trans_tlbi_data)
+  (cm : casemate_model_state) :
+  casemate_model_result :=
   let tlbi := decode_tlbi td in
   match tlbi.(TI_regime) with
-  | Regime_EL2 =>
-    (* traverse all s1 pages*)
-    traverse_si_pgt (Some tid) cm (tlbi_visitor tid tlbi) S1
-  | Regime_EL10 =>
-    (* traverse s2 pages *)
-    traverse_si_pgt (Some tid) cm (tlbi_visitor tid tlbi) S2
+  | TLBI_REGIME_EL10 =>
+    (* TLBIs that hit host/guest tables *)
+    traverse_pgt (Some tid) cm (tlbi_visitor tid tlbi) S2
+  | TLBI_REGIME_EL2 =>
+    (* TLBIs that hit pKVM's own pagetable *)
+    traverse_pgt (Some tid) cm (tlbi_visitor tid tlbi) S1
   | _ =>
-    (* traverse all page tables and add a warning *)
-    let res := traverse_all_pgt (Some tid) cm (tlbi_visitor tid tlbi) in
-    res <| cmr_log := Warning_unsupported_TLBI :: res.(cmr_log) |>
+    Merror CME_unimplemented
+    (* let res := traverse_all_pgt (Some tid) cm (tlbi_visitor tid tlbi) in
+    res <| cmr_log := Warning_unsupported_TLBI :: res.(cmr_log) |> *)
   end.
 
 (** MSR *)
@@ -1108,34 +1096,21 @@ Fixpoint root_exists (root : sm_owner_t) (roots : list cm_root) : bool :=
   | t :: q => (bool_decide (t.(r_baddr) = root)) || (root_exists root q)
   end.
 
-Definition register_root
+Definition try_register_root
   (tid : thread_identifier)
   (addr_id : addr_id_t)
   (cm : casemate_model_state)
-  (root : sm_owner_t)
+  (baddr : sm_owner_t)
   (stage : entry_stage_t) :
   casemate_model_result :=
-  let other_root_list :=
-    match stage with
-    | S1 => cmr_s2
-    | S2 => cmr_s1
-    end cm.(cms_roots) in
-  (* Check that the root does not already exist in the other root list*)
-  if root_exists root other_root_list then Merror CME_root_already_exists
-  else
-    (* Add the root to the list of roots *)
-    let new_roots :=
-      let new_root := {| r_baddr := root; r_id := addr_id; r_refcount := 0 |} in
-      match stage with
-      | S2 => cm.(cms_roots) <| cmr_s2 := new_root :: cm.(cms_roots).(cmr_s2) |>
-      | S1 => cm.(cms_roots) <| cmr_s1 := new_root :: cm.(cms_roots).(cmr_s1) |>
-      end
-    in
-    let new_st := cm <| cms_roots := new_roots |> in
-    (* then mark all its children as PTE *)
-    match root with
-    | Root r => traverse_pgt_from root r pa0 l0 stage (mark_cb tid) new_st
-    end.
+  (* Add the root to the list of roots *)
+  let new_root := {| r_baddr := baddr; r_id := addr_id; r_refcount := 0 |} in
+  let new_roots := insert_cms_root stage new_root cm.(cms_roots) in
+  let new_st := cm <| cms_roots := new_roots |> in
+  (* then mark all its children as PTE *)
+  match baddr with
+  | Root r => traverse_pgt_from baddr r pa0 l0 stage (mark_cb tid) new_st
+  end.
 
 Definition check_ttbr0_el2_asid
   (md : trans_msr_data)
@@ -1168,8 +1143,7 @@ Definition context_switch
     end in
 
   (* and increment refcount on cone we just switched to *)
-  let roots := retrieve_roots_for_stage stage decr_cm.(cms_roots) in
-  let assoc_root := retrieve_root_for_id roots addr_id in
+  let assoc_root := retrieve_root_for_id stage decr_cm.(cms_roots) addr_id in
   match assoc_root with
   | Some root =>
     let new_assoc_root := {| 
@@ -1178,48 +1152,50 @@ Definition context_switch
       r_refcount := root.(r_refcount) + 1 |} in
     let new_cms_roots := update_cms_root_for_id stage (root.(r_id)) new_assoc_root cm.(cms_roots) in
     let incr_cm := decr_cm <| cms_roots := new_cms_roots |> in
-    (* update the current context *)
+    (* make it the curent context *)
     let final_cm := update_current_thread_context tid stage root.(r_baddr) incr_cm in
     Mreturn final_cm
   | None => Merror (CME_internal_error IET_unexpected_none)
   end.
-  
+
+Definition stage_from_ttbr
+  (sysreg : ghost_sysreg_kind) : entry_stage_t :=
+  match sysreg with
+  | SYSREG_TTBR_EL2 => S1
+  | SYSREG_VTTBR => S2
+  end.
+
 Definition step_msr 
   (tid : thread_identifier)
   (md : trans_msr_data)
   (cm : casemate_model_state) : 
   casemate_model_result :=
-  let stage :=
-    match md.(tmd_sysreg) with
-    | SYSREG_TTBR_EL2 => S1
-    | SYSREG_VTTBR => S2
-    end
-  in
-  let root := ttbr_extract_baddr md.(tmd_val) in
+  let stage := stage_from_ttbr md.(tmd_sysreg) in
+  let baddr := ttbr_extract_baddr md.(tmd_val) in
   let addr_id := ttbr_extract_id md.(tmd_val) in
+
   (* TTBR0_EL2 in non-VHE mode has a Res0 ASID *)
   if negb (check_ttbr0_el2_asid md addr_id) then
     Merror (CME_addr_id_error "TTBR0_EL2 ASID is reserved 0")
   else
-    let roots := retrieve_roots_for_stage stage cm.(cms_roots) in
-    match retrieve_root_for_baddr roots root with
+    match retrieve_root_for_baddr stage cm.(cms_roots) baddr with
     | Some assoc_root =>
       (* if that root with that id exists already, were just context switching *)
       if (bool_decide (assoc_root.(r_id) = addr_id)) then
         context_switch tid addr_id stage md cm
       else
-      (* see if that root is already associated with a different (VM/AS)ID *)
+        (* see if that root is already associated with a different (VM/AS)ID *)
         Merror (CME_addr_id_error "root already associated with an (VM/AS)ID")
     | None =>
       let res :=
-        match retrieve_root_for_id roots addr_id with
+        match retrieve_root_for_id stage cm.(cms_roots) addr_id with
         | Some assoc_root =>
-          if negb (bool_decide (assoc_root.(r_baddr) = root)) then
+          if negb (bool_decide (assoc_root.(r_baddr) = baddr)) then
             Merror (CME_addr_id_error "duplicate (VM/AS)ID")
           else if negb (bool_decide (assoc_root.(r_id) = addr_id)) then
             Merror (CME_addr_id_error "root already associated with an (VM/AS)ID")
-          else register_root tid addr_id cm root stage
-        | None => register_root tid addr_id cm root stage
+          else try_register_root tid addr_id cm baddr stage
+        | None => try_register_root tid addr_id cm baddr stage
         end in
       match res.(cmr_data) with
       | Ok _ _ cm => context_switch tid addr_id stage md cm
@@ -1259,7 +1235,7 @@ Function set_owner_root
       let new_pte :=
         match location.(sl_pte) with
         | None => None
-        | Some pte => Some (pte <| ged_owner := root|>) (* actually change the root *)
+        | Some pte => Some (pte <| eed_owner := root|>) (* actually change the root *)
         end
       in
       (* Write the change to the global state *)
@@ -1279,7 +1255,7 @@ Definition step_release_cb (ctx : pgtable_traverse_context) : casemate_model_res
     match location.(sl_pte) with
     | None => Merror (CME_not_a_pte "release_cb" ctx.(ptc_addr))
     | Some desc =>
-      match desc.(ged_state) with
+      match desc.(eed_state) with
       | SPS_STATE_PTE_INVALID_UNCLEAN _ =>
           Merror (CME_bbm_violation VT_release_unclean ctx.(ptc_addr))
       | _ => Mreturn ctx.(ptc_state)
@@ -1317,13 +1293,13 @@ Definition try_unregister_root
     | None => Merror (CME_internal_error IET_unexpected_none)
     | Some pte =>
       let new_roots :=
-        match pte.(ged_stage) with
+        match pte.(eed_stage) with
         | S2 => cm.(cms_roots) <| cmr_s2 := unregister_root addr [] cm.(cms_roots).(cmr_s2) |>
         | S1 => cm.(cms_roots) <| cmr_s1 := unregister_root addr [] cm.(cms_roots).(cmr_s1) |>
         end
       in
       let cm := cm <| cms_roots := new_roots |> in
-      traverse_pgt_from_root addr pte.(ged_stage) (unmark_cb cpu) cm
+      traverse_pgt_from_root addr pte.(eed_stage) (unmark_cb cpu) cm
     end
   end.
 
@@ -1340,10 +1316,10 @@ Definition step_release_table
     | Some desc =>
       let new_st := traverse_pgt_from
         addr
-        (root_val desc.(ged_owner))
-        desc.(ged_ia_region).(range_start)
-        desc.(ged_level)
-        desc.(ged_stage)
+        (root_val desc.(eed_owner))
+        desc.(eed_ia_region).(range_start)
+        desc.(eed_level)
+        desc.(eed_stage)
         step_release_cb
         cm in
       Mupdate_state (try_unregister_root (addr) cpu) new_st
@@ -1362,7 +1338,7 @@ Definition step_hint_set_pte_thread_owner
     match location.(sl_pte) with
     | None => Merror (CME_not_a_pte "set_pte_thread_owner"%string phys)
     | Some _ =>
-      let thread_owner := TID (to_nat (phys_addr_val (root_val val))) in
+      let thread_owner := TID (phys_addr_val (root_val val)) in
       Mreturn (cm <| cms_memory :=
         (<[ location.(sl_phys_addr) := location <| sl_thread_owner := Some thread_owner |> ]> cm.(cms_memory))
       |> )
